Lean4Lean/Theory.lean
@@ -2,3 +2,4 @@ import Lean4Lean.Theory.Typing.EnvLemmas
 import Lean4Lean.Theory.Typing.Strong
 import Lean4Lean.Theory.Typing.UniqueTyping
 import Lean4Lean.Theory.Typing.ChurchRosser
+import Lean4Lean.Theory.Typing.HeadReduction
