Lean4Lean/Theory/Typing/HeadReduction.lean
@@ -1,0 +1,480 @@
+import Lean4Lean.Theory.Typing.ChurchRosser
+
+/-!
+
+# Theorems about (weak) head reduction
+
+This includes the proof of the Standardization theorem, based on a proof by Kashima (2000):
+Ryo Kashima, "A Proof of the Standardization Theorem in λ-Calculus"
+<https://www.is.c.titech.ac.jp/~kashima/pub/C-145.pdf>.
+
+-/
+
+namespace Lean4Lean
+namespace VEnv
+
+open VExpr
+variable [Params]
+open Params
+
+local notation:65 Γ " ⊢ " e " : " A:36 => HasType env univs Γ e A
+local notation:65 Γ " ⊢ " e1 " ≡ " e2:36 " : " A:36 => IsDefEq env univs Γ e1 e2 A
+local notation:65 Γ " ⊢ " e1 " ≡ " e2:36 => IsDefEqU env univs Γ e1 e2
+local notation:65 Γ " ⊢ " e1 " ≫ " e2:36 => ParRed Γ e1 e2
+local notation:65 Γ " ⊢ " e1 " ≫* " e2:36 => ParRedS Γ e1 e2
+
+omit [Params] in
+theorem Subpattern.varN_const (H : Subpattern p (.varN (.const c) n)) :
+    ∃ n, p = .varN (.const c) n := by
+  generalize eq : Pattern.varN (.const c) n = p' at H
+  induction H generalizing n with
+  | refl => exact ⟨_, eq.symm⟩
+  | appL | appR => cases n <;> cases eq
+  | varL _ ih => cases n <;> cases eq; exact ih rfl
+
+theorem Params.simple_app (H : Pat p r) (h : Subpattern (.app p₁ p₂) p) : .app p₁ p₂ = p := by
+  obtain ⟨_|_, rfl⟩ := pat_simple H <;> cases h
+  · rfl
+  · obtain ⟨_|_, ⟨⟩⟩ := Subpattern.varN_const ‹_›
+  · obtain ⟨_|_, ⟨⟩⟩ := Subpattern.varN_const ‹_›
+
+def IsMajorPremise (e : VExpr) :=
+  ∃ p, (∃ r, Pat p r) ∧ ∃ p₁ p₂, Subpattern (.app p₁ p₂) p ∧ ∃ m1 m2, p₁.Matches e m1 m2
+
+theorem IsMajorPremise.lift' {e ρ} : IsMajorPremise (e.lift' ρ) ↔ IsMajorPremise e := by
+  constructor <;> intro ⟨_, h1, _, _, h2, _, _, h3⟩
+  · let ⟨_, h4, _⟩ := Pattern.matches_lift'.1 h3
+    exact ⟨_, h1, _, _, h2, _, _, h4⟩
+  · exact ⟨_, h1, _, _, h2, _, _, Pattern.matches_lift'.2 ⟨_, h3, fun _ => rfl⟩⟩
+
+theorem IsMajorPremise.instN : IsMajorPremise e1 → IsMajorPremise (e1.inst a k)
+  | ⟨_, h1, _, _, h2, _, _, h3⟩ => ⟨_, h1, _, _, h2, _, _, Pattern.matches_instN h3⟩
+
+theorem IsMajorPremise.lam : ¬IsMajorPremise (.lam A e) := nofun
+
+set_option hygiene false
+local notation:65 Γ " ⊢ " e1 " ⤳ " e2:36 => WHRed Γ e1 e2
+inductive WHRed (Γ : List VExpr) : VExpr → VExpr → Prop where
+  | app : Γ ⊢ f ⤳ f' → Γ ⊢ .app f a ⤳ .app f' a
+  | major : IsMajorPremise f → Γ ⊢ a ⤳ a' → Γ ⊢ .app f a ⤳ .app f a'
+  | beta : Γ ⊢ .app (.lam A e) a ⤳ e.inst a
+  | extra : Pat p r → p.Matches e m1 m2 → r.2.OK (IsDefEqU env univs Γ) m1 m2 →
+    Γ ⊢ e ⤳ r.1.apply m1 m2
+
+theorem WHRed.defeqDFC (W : IsDefEqCtx env univs Γ₀ Γ₁ Γ₂)
+    (H : Γ₁ ⊢ e1 ⤳ e2) : Γ₂ ⊢ e1 ⤳ e2 := by
+  induction H generalizing Γ₂ with
+  | app _ ih1 => exact .app (ih1 W)
+  | major h1 _ ih1 => exact .major h1 (ih1 W)
+  | beta => exact .beta
+  | extra h1 h2 h3 => exact .extra h1 h2 <| h3.map fun a b h => h.defeqDFC henv W
+
+theorem WHRed.weak' (W : Ctx.Lift' ρ Γ Γ') :
+    Γ ⊢ e1 ⤳ e2 → Γ' ⊢ e1.lift' ρ ⤳ e2.lift' ρ
+  | .app h1 => .app (h1.weak' W)
+  | .major h1 h2 => .major (IsMajorPremise.lift'.2 h1) (h2.weak' W)
+  | .beta => by rw [VExpr.lift'_inst_hi]; exact .beta
+  | .extra h1 h2 h3 => by
+    rw [Pattern.RHS.apply_lift']
+    refine .extra h1 (Pattern.matches_lift'.2 ⟨_, h2, fun _ => rfl⟩) <| h3.map fun _ _ h => ?_
+    simp only [← Pattern.RHS.apply_lift']; exact h.weak' henv W
+
+theorem WHRed.weakN (W : Ctx.LiftN n k Γ Γ') (H : Γ ⊢ e1 ⤳ e2) :
+    Γ' ⊢ e1.liftN n k ⤳ e2.liftN n k := by
+  simp only [← lift'_consN_skipN]; exact H.weak' (Ctx.liftN_iff_lift'.1 W)
+
+variable! (hΓ : OnCtx Γ' (IsType env univs)) in
+theorem WHRed.weakU_inv (W : Ctx.Lift' ρ Γ Γ') (H : Γ' ⊢ e1.lift' ρ ⤳ e2') :
+    ∃ e2, e2' = e2.lift' ρ ∧ Γ ⊢ e1 ⤳ e2 := by
+  generalize he : e1.lift' ρ = e1' at H
+  induction H generalizing e1 with
+  | app h1 ih => let .app .. := e1; cases he; obtain ⟨_, rfl, a1⟩ := ih rfl; exact ⟨_, rfl, .app a1⟩
+  | major h1 h2 ih =>
+    let .app .. := e1; cases he; obtain ⟨_, rfl, a1⟩ := ih rfl
+    exact ⟨_, rfl, .major (IsMajorPremise.lift'.1 h1) a1⟩
+  | beta =>
+    let .app e1 _ := e1; let .lam .. := e1; cases he
+    simp [← VExpr.lift'_inst_hi, VExpr.lift'_inj]; exact .beta
+  | extra h1 h2 h3 =>
+    subst he
+    obtain ⟨_, h4, h5⟩ := Pattern.matches_lift'.1 h2; cases funext h5
+    refine ⟨_, (Pattern.RHS.apply_lift' _).symm, .extra h1 h4 <| h3.map fun _ _ h => ?_⟩
+    simp only [← Pattern.RHS.apply_lift'] at h
+    exact (IsDefEqU.weak'_iff henv hΓ W).1 h
+
+theorem WHRed.parRed (H : Γ ⊢ e1 ⤳ e2) : Γ ⊢ e1 ≫ e2 := by
+  induction H with
+  | app _ ih => exact .app ih .rfl
+  | major _ _ ih => exact .app .rfl ih
+  | beta => exact .beta .rfl .rfl
+  | extra h1 h2 h3 => exact .extra h1 h2 h3 fun _ => .rfl
+
+variable! (hΓ : OnCtx Γ (IsType env univs)) in
+theorem WHRed.defeq (H : Γ ⊢ e1 ⤳ e2) (he : Γ ⊢ e1 : A) : Γ ⊢ e1 ≡ e2 : A :=
+  H.parRed.defeq hΓ he
+
+variable! (hΓ : OnCtx Γ (IsType env univs)) in
+theorem WHRed.hasType (H : Γ ⊢ e1 ⤳ e2) (he : Γ ⊢ e1 : A) : Γ ⊢ e2 : A := (H.defeq hΓ he).hasType.2
+
+variable! (H₀ : Γ₀ ⊢ a : A₀) in
+theorem WHRed.instN (W : Ctx.InstN Γ₀ a A₀ k Γ₁ Γ)
+    (H : Γ₁ ⊢ e1 ⤳ e2) : Γ ⊢ e1.inst a k ⤳ e2.inst a k := by
+  induction H with
+  | app _ ih => exact .app ih
+  | major h1 _ ih => exact .major h1.instN ih
+  | beta => rw [(by apply inst_inst_hi : (inst ..).inst _ _ = _)]; exact .beta
+  | extra h1 h2 h3 =>
+    rw [Pattern.RHS.instN_apply]
+    exact .extra h1 (Pattern.matches_instN h2) (h3.instN W H₀)
+
+def WHNF (Γ : List VExpr) (e : VExpr) := ∀ e', ¬Γ ⊢ e ⤳ e'
+
+theorem WHNF.bvar : WHNF Γ (.bvar i) := nofun
+theorem WHNF.lam : WHNF Γ (.lam A e) := nofun
+theorem WHNF.sort : WHNF Γ (.sort A) := nofun
+theorem WHNF.forallE : WHNF Γ (.forallE A B) := nofun
+
+theorem WHNF.subpattern
+    (h1 : Pat p r) (h2 : Subpattern p₁ p) (h3 : p₁ ≠ p) (h4 : p₁.Matches e m1 m2) : WHNF Γ e := by
+  intro _ H2
+  obtain ⟨c, n, rfl⟩ : ∃ c n, p₁ = .varN (.const c) n := by
+    obtain ⟨_|_, rfl⟩ := pat_simple h1 <;> cases h2 <;>
+      first | cases h3 rfl | exact ⟨_, Subpattern.varN_const ‹_›⟩
+  have : ∀ r, ¬Pat (.const c) r := fun _ h => by
+    cases (pat_uniq h1 h (.trans (.varN .refl) h2) (Pattern.inter_self _)).1
+    exact h3.symm (h2.antisymm (.varN .refl))
+  clear h3
+  induction H2 generalizing n with
+  | app r1 ih => let n+1 := n; let .var h4 := h4; exact ih _ (.trans (.varL .refl) h2) h4
+  | major r1 r2 ih =>
+    let n+1 := n; let .var h4 := h4
+    let ⟨p', ⟨_, h1'⟩, p₁', p₂', h2', _, _, h3'⟩ := r1
+    cases simple_app h1' h2'
+    obtain ⟨⟨_, n, _⟩ | _, rfl⟩ := pat_simple h1 <;> [skip; cases n <;> cases h2]
+    have ⟨_, _, _, a1, a2⟩ := Pattern.matches_inter.1 ⟨⟨_, _, h3'⟩, ⟨_, _, h4⟩⟩
+    cases h2 with
+    | appL h2 => cases (pat_app_l_uniq h1 h1' .refl .refl h2).symm.trans a1
+    | appR h2 =>
+      cases (pat_app_uniq h1' h1 .refl .refl .refl (.trans (.varL .refl) h2)).symm.trans a1
+  | beta => generalize Pattern.varN .. = p' at m1 m2 h4; nomatch h4
+  | extra r1 r2 r3 =>
+    have ⟨_, _, _, a1, a2⟩ := Pattern.matches_inter.1 ⟨⟨_, _, r2⟩, ⟨_, _, h4⟩⟩
+    obtain ⟨⟨_, m, _⟩ | _, rfl⟩ := pat_simple h1 <;> [skip; cases n <;> cases h2]
+    obtain ⟨rfl, eq, _⟩ := pat_uniq h1 r1 h2 a1
+    cases n <;> cases eq
+    exact this _ h1
+
+theorem IsMajorPremise.whnf : IsMajorPremise e → WHNF Γ e := by
+  rintro ⟨p, ⟨_, h1⟩, p₁, p₂, h2, _, _, h3⟩
+  refine .subpattern h1 (.trans (.appL .refl) h2) ?_ h3
+  rintro rfl; cases h2.antisymm (.appL .refl)
+
+theorem WHRed.determ (H1 : Γ ⊢ e ⤳ e₁) (H2 : Γ ⊢ e ⤳ e₂) : e₁ = e₂ := by
+  induction H1 generalizing e₂ with
+  | app l1 ih =>
+    cases H2 with
+    | app r1 => cases ih r1; rfl
+    | major r1 r2 => cases r1.whnf _ l1
+    | beta => cases WHNF.lam _ l1
+    | extra r1 r2 =>
+      cases r2 with
+      | app r3 => cases IsMajorPremise.whnf ⟨_, ⟨_, r1⟩, _, _, .refl, _, _, r3⟩ _ l1
+      | var => cases pat_not_var r1
+  | major l1 l2 ih =>
+    cases H2 with
+    | app r1 => cases l1.whnf _ r1
+    | major _ r2 => cases ih r2; rfl
+    | beta => cases l1.lam
+    | extra r1 r2 =>
+      cases r2 with
+      | var => cases pat_not_var r1
+      | app _ r4 => cases WHNF.subpattern r1 (.appR .refl) nofun r4 _ l2
+  | beta =>
+    cases H2 with
+    | app r1 => cases WHNF.lam _ r1
+    | major r1 => cases r1.lam
+    | beta => rfl
+    | extra _ r2 => nomatch r2
+  | extra l1 l2 =>
+    cases H2 with
+    | beta => nomatch l2
+    | major r1 r2 =>
+      cases l2 with
+      | var => cases pat_not_var l1
+      | app _ l4 => cases WHNF.subpattern l1 (.appR .refl) nofun l4 _ r2
+    | app r1 =>
+      cases l2 with
+      | app l3 => cases IsMajorPremise.whnf ⟨_, ⟨_, l1⟩, _, _, .refl, _, _, l3⟩ _ r1
+      | var => cases pat_not_var l1
+    | extra r1 r2 =>
+      have ⟨_, _, _, a1, a2⟩ := Pattern.matches_inter.1 ⟨⟨_, _, r2⟩, ⟨_, _, l2⟩⟩
+      obtain ⟨rfl, -, ⟨⟩⟩ := pat_uniq l1 r1 .refl a1
+      obtain ⟨rfl, rfl⟩ := Pattern.matches_determ l2 r2; rfl
+
+def WHRedS (Γ : List VExpr) : VExpr → VExpr → Prop := ReflTransGen (WHRed Γ)
+local notation:65 Γ " ⊢ " e1 " ⤳* " e2:36 => WHRedS Γ e1 e2
+
+theorem WHRedS.defeqDFC (W : IsDefEqCtx env univs Γ₀ Γ₁ Γ₂)
+    (H : Γ₁ ⊢ e1 ⤳* e2) : Γ₂ ⊢ e1 ⤳* e2 := by
+  induction H with
+  | rfl => exact .rfl
+  | tail _ h2 ih => exact .tail ih (h2.defeqDFC W)
+
+theorem WHRedS.parRedS (H : Γ ⊢ e1 ⤳* e2) : Γ ⊢ e1 ≫* e2 := by
+  induction H with
+  | rfl => exact .rfl
+  | tail _ h2 ih => exact .tail ih h2.parRed
+
+theorem WHRedS.app (H : Γ ⊢ f ⤳* f') : Γ ⊢ f.app a ⤳* f'.app a := by
+  induction H with
+  | rfl => exact .rfl
+  | tail _ h2 ih => exact .tail ih h2.app
+
+theorem WHRedS.major (H1 : IsMajorPremise f) (H : Γ ⊢ a ⤳* a') : Γ ⊢ f.app a ⤳* f.app a' := by
+  induction H with
+  | rfl => exact .rfl
+  | tail _ h2 ih => exact .tail ih (h2.major H1)
+
+variable! (hΓ : OnCtx Γ (IsType env univs)) in
+theorem WHRedS.defeq (H : Γ ⊢ e1 ⤳* e2) (he : Γ ⊢ e1 : A) : Γ ⊢ e1 ≡ e2 : A :=
+  H.parRedS.defeq hΓ he
+
+variable! (hΓ : OnCtx Γ (IsType env univs)) in
+theorem WHRedS.hasType (H : Γ ⊢ e1 ⤳* e2) (he : Γ ⊢ e1 : A) : Γ ⊢ e2 : A :=
+  (H.defeq hΓ he).hasType.2
+
+theorem WHRedS.weak' (W : Ctx.Lift' ρ Γ Γ')
+    (H : Γ ⊢ e1 ⤳* e2) : Γ' ⊢ e1.lift' ρ ⤳* e2.lift' ρ := by
+  induction H with
+  | rfl => exact .rfl
+  | tail _ h2 ih => exact .tail ih (h2.weak' W)
+
+theorem WHRedS.weakN (W : Ctx.LiftN n k Γ Γ') (H : Γ ⊢ e1 ⤳* e2) :
+    Γ' ⊢ e1.liftN n k ⤳* e2.liftN n k := by
+  simp only [← lift'_consN_skipN]; exact H.weak' (Ctx.liftN_iff_lift'.1 W)
+
+theorem WHRedS.instN (H₀ : Γ₀ ⊢ a : A₀) (W : Ctx.InstN Γ₀ a A₀ k Γ₁ Γ)
+    (H : Γ₁ ⊢ e1 ⤳* e2) : Γ ⊢ e1.inst a k ⤳* e2.inst a k := by
+  induction H with
+  | rfl => exact .rfl
+  | tail _ h2 ih => exact .tail ih (h2.instN H₀ W)
+
+theorem WHNF.whRedS (H : WHNF Γ e) (H2 : Γ ⊢ e ⤳* e') : e = e' := by
+  cases H2 using ReflTransGen.headIndOn with
+  | rfl => rfl
+  | head h1 => cases H _ h1
+
+local notation:65 Γ " ⊢ " e1 " ⤳< " e2:36 => StRed Γ e1 e2
+inductive StRed : List VExpr → VExpr → VExpr → Prop where
+  | bvar : Γ ⊢ e ⤳* .bvar i → Γ ⊢ e ⤳< .bvar i
+  | sort : Γ ⊢ e ⤳* .sort u → Γ ⊢ e ⤳< .sort u
+  | const : Γ ⊢ e ⤳* .const c ls → Γ ⊢ e ⤳< .const c ls
+  | app : Γ ⊢ e ⤳* .app f a → Γ ⊢ f ⤳< f' → Γ ⊢ a ⤳< a' → Γ ⊢ e ⤳< .app f' a'
+  | lam : Γ ⊢ e ⤳* .lam A body → Γ ⊢ A ⤳< A' → A::Γ ⊢ body ⤳< body' → Γ ⊢ e ⤳< .lam A' body'
+  | forallE : Γ ⊢ e ⤳* .forallE A B → Γ ⊢ A ⤳< A' → A::Γ ⊢ B ⤳< B' → Γ ⊢ e ⤳< .forallE A' B'
+
+protected theorem StRed.rfl : ∀ {e}, Γ ⊢ e ⤳< e
+  | .bvar _ => .bvar .rfl
+  | .sort .. => .sort .rfl
+  | .const .. => .const .rfl
+  | .app .. => .app .rfl .rfl .rfl
+  | .lam .. => .lam .rfl .rfl .rfl
+  | .forallE .. => .forallE .rfl .rfl .rfl
+
+theorem StRed.bvar_l (H : Γ ⊢ .bvar i ⤳< e) : e = .bvar i := by
+  cases H with
+  | bvar h1 | sort h1 | const h1 | app h1 | lam h1 | forallE h1 => cases WHNF.bvar.whRedS h1 <;> rfl
+
+theorem StRed.sort_l (H : Γ ⊢ .sort u ⤳< e) : e = .sort u := by
+  cases H with
+  | bvar h1 | sort h1 | const h1 | app h1 | lam h1 | forallE h1 => cases WHNF.sort.whRedS h1 <;> rfl
+
+theorem StRed.lam_l (H : Γ ⊢ .lam A B ⤳< e) :
+    ∃ A' B', e = .lam A' B' ∧ Γ ⊢ A ⤳< A' ∧ A::Γ ⊢ B ⤳< B' := by
+  cases H with
+  | bvar h1 | sort h1 | const h1 | app h1 | forallE h1 => cases WHNF.lam.whRedS h1
+  | lam h1 h2 h3 => cases WHNF.lam.whRedS h1; exact ⟨_, _, rfl, h2, h3⟩
+
+theorem StRed.forallE_l (H : Γ ⊢ .forallE A B ⤳< e) :
+    ∃ A' B', e = .forallE A' B' ∧ Γ ⊢ A ⤳< A' ∧ A::Γ ⊢ B ⤳< B' := by
+  cases H with
+  | bvar h1 | sort h1 | const h1 | app h1 | lam h1 => cases WHNF.forallE.whRedS h1
+  | forallE h1 h2 h3 => cases WHNF.forallE.whRedS h1; exact ⟨_, _, rfl, h2, h3⟩
+
+variable! (hΓ₀ : OnCtx Γ₀ (IsType env univs)) in
+theorem StRed.defeqDFC (W : IsDefEqCtx env univs Γ₀ Γ₁ Γ₂)
+    (h : Γ₁ ⊢ e1 : A) (H : Γ₁ ⊢ e1 ⤳< e2) : Γ₂ ⊢ e1 ⤳< e2 := by
+  induction H generalizing Γ₂ A with
+  | bvar h1 => exact .bvar (h1.defeqDFC W)
+  | sort h1 => exact .sort (h1.defeqDFC W)
+  | const h1 => exact .const (h1.defeqDFC W)
+  | app h1 _ _ ih1 ih2 =>
+    let hΓ := W.isType' hΓ₀; have ⟨_, _, hf, ha⟩ := (h1.hasType hΓ h).app_inv henv hΓ
+    exact .app (h1.defeqDFC W) (ih1 W hf) (ih2 W ha)
+  | lam h1 _ _ ih1 ih2 =>
+    let hΓ := W.isType' hΓ₀; have ⟨⟨_, hA⟩, _, he⟩ := (h1.hasType hΓ h).lam_inv henv hΓ
+    exact .lam (h1.defeqDFC W) (ih1 W hA) (ih2 (W.succ hA) he)
+  | forallE h1 _ _ ih1 ih2 =>
+    let hΓ := W.isType' hΓ₀; have ⟨⟨_, hA⟩, _, hB⟩ := (h1.hasType hΓ h).forallE_inv henv
+    exact .forallE (h1.defeqDFC W) (ih1 W hA) (ih2 (W.succ hA) hB)
+
+theorem StRed.parRedS (H : Γ ⊢ e ⤳< e') : Γ ⊢ e ≫* e' := by
+  induction H with
+  | bvar h1 | sort h1 | const h1 => exact h1.parRedS
+  | app h1 _ _ ih1 ih2 => exact h1.parRedS.trans (ih1.app ih2)
+  | lam h1 _ _ ih1 ih2 => exact h1.parRedS.trans (ih1.lam ih2)
+  | forallE h1 _ _ ih1 ih2 => exact h1.parRedS.trans (ih1.forallE ih2)
+
+theorem StRed.whRed (H1 : Γ ⊢ e₁ ⤳* e₂) (H2 : Γ ⊢ e₂ ⤳< e') : Γ ⊢ e₁ ⤳< e' := by
+  cases H2 with
+  | bvar h1 => exact .bvar (H1.trans h1)
+  | sort h1 => exact .sort (H1.trans h1)
+  | const h1 => exact .const (H1.trans h1)
+  | app h1 h2 h3 => exact .app (H1.trans h1) h2 h3
+  | lam h1 h2 h3 => exact .lam (H1.trans h1) h2 h3
+  | forallE h1 h2 h3 => exact .forallE (H1.trans h1) h2 h3
+
+variable! (hΓ : OnCtx Γ (IsType env univs)) in
+theorem StRed.defeq (H : Γ ⊢ e1 ⤳< e2) (he : Γ ⊢ e1 : A) : Γ ⊢ e1 ≡ e2 : A :=
+  H.parRedS.defeq hΓ he
+
+theorem StRed.weak' (W : Ctx.Lift' ρ Γ Γ') (H : Γ ⊢ e1 ⤳< e2) :
+    Γ' ⊢ e1.lift' ρ ⤳< e2.lift' ρ := by
+  induction H generalizing ρ Γ' with
+  | bvar h1 => exact .bvar (h1.weak' W)
+  | sort h1 => exact .sort (h1.weak' W)
+  | const h1 => exact .const (h1.weak' W)
+  | app h1 _ _ ih1 ih2 => exact .app (h1.weak' W) (ih1 W) (ih2 W)
+  | lam h1 _ _ ih1 ih2 => exact .lam (h1.weak' W) (ih1 W) (ih2 W.cons)
+  | forallE h1 _ _ ih1 ih2 => exact .forallE (h1.weak' W) (ih1 W) (ih2 W.cons)
+
+theorem StRed.weakN (W : Ctx.LiftN n k Γ Γ') (H : Γ ⊢ e1 ⤳< e2) :
+    Γ' ⊢ e1.liftN n k ⤳< e2.liftN n k := by
+  simp only [← lift'_consN_skipN]; exact H.weak' (Ctx.liftN_iff_lift'.1 W)
+
+variable! (H₀ : Γ₀ ⊢ a1 ⤳< a2) (H₀' : Γ₀ ⊢ a1 : A₀) in
+theorem StRed.instN (W : Ctx.InstN Γ₀ a1 A₀ k Γ₁ Γ)
+    (H : Γ₁ ⊢ e1 ⤳< e2) : Γ ⊢ e1.inst a1 k ⤳< e2.inst a2 k := by
+  induction H generalizing Γ k with
+  | @bvar _ e i h1 =>
+    refine .whRed (h1.instN H₀' W) ?_; clear h1
+    induction W generalizing i with
+    | zero =>
+      cases i with simp [inst]
+      | zero => exact .whRed .rfl H₀
+      | succ i => exact .bvar .rfl
+    | succ _ ih =>
+      cases i with simp [inst]
+      | zero => exact .bvar .rfl
+      | succ h => exact ih.weakN .one
+  | sort h1 => exact .sort (h1.instN H₀' W)
+  | const h1 => exact .const (h1.instN H₀' W)
+  | app h1 _ _ ih1 ih2 => exact .app (h1.instN H₀' W) (ih1 W) (ih2 W)
+  | lam h1 _ _ ih1 ih2 => exact .lam (h1.instN H₀' W) (ih1 W) (ih2 W.succ)
+  | forallE h1 _ _ ih1 ih2 => exact .forallE (h1.instN H₀' W) (ih1 W) (ih2 W.succ)
+
+theorem StRed.apply_pat {p : Pattern} (r : p.RHS) {m1 m2 m3}
+    (H : ∀ a, Γ ⊢ m2 a ⤳< m3 a) : Γ ⊢ r.apply m1 m2 ⤳< r.apply m1 m3 := by
+  match r with
+  | .fixed .. => exact .rfl
+  | .app f a => exact .app .rfl (apply_pat f H) (apply_pat a H)
+  | .var f => exact H _
+
+variable! (hΓ₀ : OnCtx Γ₀ (IsType env univs)) in
+theorem StRed.triangle (W : IsDefEqCtx env univs Γ₀ Γ₁ Γ₂)
+    (h : Γ₁ ⊢ e : A) (H1 : Γ₁ ⊢ e ⤳< e₁) (H2 : Γ₂ ⊢ e₁ ≫ e₂) : Γ₁ ⊢ e ⤳< e₂ := by
+  induction H2 generalizing Γ₁ e A with
+  | bvar | sort | const => exact H1
+  | app b1 b2 ih1 ih2 =>
+    let .app a1 a2 a3 := H1
+    have hΓ := W.isType' hΓ₀; have ⟨_, _, hf, ha⟩ := (a1.hasType hΓ h).app_inv henv hΓ
+    exact .app a1 (ih1 W hf a2) (ih2 W ha a3)
+  | lam b1 b2 ih1 ih2 =>
+    let .lam a1 a2 a3 := H1
+    have hΓ := W.isType' hΓ₀; have ⟨⟨_, hA⟩, _, he⟩ := (a1.hasType hΓ h).lam_inv henv hΓ
+    exact .lam a1 (ih1 W hA a2) (ih2 (W.succ (a2.defeq hΓ hA)) he.hasType.1 a3)
+  | forallE b1 b2 ih1 ih2 =>
+    let .forallE a1 a2 a3 := H1
+    have hΓ := W.isType' hΓ₀; have ⟨⟨_, hA⟩, _, he⟩ := (a1.hasType hΓ h).forallE_inv henv
+    exact .forallE a1 (ih1 W hA a2) (ih2 (W.succ (a2.defeq hΓ hA)) he.hasType.1 a3)
+  | beta _ _ ih1 ih2 =>
+    let .app a1 a2 a3 := H1; let .lam a4 a5 a6 := a2
+    have hΓ := W.isType' hΓ₀; have ⟨_, _, hf, ha⟩ := (a1.hasType hΓ h).app_inv henv hΓ
+    have c1 := a4.hasType hΓ hf; have ⟨⟨_, hA⟩, _, he⟩ := c1.lam_inv henv hΓ
+    have ⟨⟨_, u1⟩, _, u2⟩ := (c1.uniqU henv hΓ (hA.lam he)).forallE_inv henv hΓ
+    exact .whRed (a1.trans a4.app |>.tail .beta) <|
+      (ih2 W ha a3).instN (u1.defeq ha) .zero (ih1 (W.succ (a5.defeq hΓ hA)) he a6)
+  | @extra p r e₁ m1 m2 Γ₂ m2' h1 h2 h3 _ ih =>
+    have hΓ := W.isType' hΓ₀
+    suffices ∀ p' m1 m2, Subpattern p' p → p'.Matches e₁ m1 m2 →
+         ∃ e₁ m3, Γ₁ ⊢ e ⤳* e₁ ∧ p'.Matches e₁ m1 m3 ∧ (∀ x, Γ₁ ⊢ m3 x ⤳< m2 x) by
+      let ⟨e₁, m3, a1, a2, a3⟩ := this _ _ _ .refl h2
+      have := (a1.hasType hΓ h).matches_inv hΓ a2
+      refine .whRed (.tail a1 (.extra h1 a2 <| h3.map fun a b ⟨_, h⟩ => ?_))
+        (.apply_pat _ fun x => let ⟨_, h⟩ := this x; ih x W h (a3 x))
+      replace h := h.defeqDFC henv (W.symm henv)
+      refine have {r} := IsDefEq.apply_pat hΓ (r := r) fun a A h => ?_
+        ⟨_, (this h.hasType.1).symm.trans <| h.trans (this h.hasType.2)⟩
+      let ⟨_, h'⟩ := this a; exact ⟨_, ((a3 a).defeq hΓ h').symm⟩
+    clear h2 ih h; intro p' m1 m2 hp h2
+    induction h2 generalizing e with
+    | const => let .const H1 := H1; exact ⟨_, _, H1, .const, nofun⟩
+    | app l1 l2 ih1 ih2 =>
+      let .app r1 r2 r3 := H1
+      have ⟨_, _, a1, a2, a3⟩ := ih1 r2 (.trans (.appL .refl) hp)
+      have ⟨_, _, b1, b2, b3⟩ := ih2 r3 (.trans (.appR .refl) hp)
+      refine ⟨_, _, r1.trans a1.app |>.trans (b1.major ?_), .app a2 b2, (·.casesOn a3 b3)⟩
+      exact ⟨_, ⟨_, h1⟩, _, _, hp, _, _, a2⟩
+    | var l1 ih1 =>
+      let .app r1 r2 r3 := H1
+      have ⟨_, _, a1, a2, a3⟩ := ih1 r2 (.trans (.varL .refl) hp)
+      refine ⟨_, _, r1.trans a1.app, .var a2, (·.casesOn r3 a3)⟩
+
+variable! (hΓ₀ : OnCtx Γ₀ (IsType env univs)) in
+theorem StRed.triangleS (W : IsDefEqCtx env univs Γ₀ Γ₁ Γ₂)
+    (h : Γ₁ ⊢ e : A) (H1 : Γ₁ ⊢ e ⤳< e₁) (H2 : Γ₂ ⊢ e₁ ≫* e₂) : Γ₁ ⊢ e ⤳< e₂ := by
+  induction H2 with
+  | rfl => exact H1
+  | tail _ h2 ih => exact ih.triangle hΓ₀ W h h2
+
+variable! (hΓ : OnCtx Γ (IsType env univs)) in
+theorem ParRedS.standard (h : Γ ⊢ e : A) (H : Γ ⊢ e ≫* e') : Γ ⊢ e ⤳< e' :=
+  .triangleS hΓ .zero h .rfl H
+
+variable! (hΓ : OnCtx Γ (IsType env univs)) in
+theorem IsDefEq.reduce_sort (H : Γ ⊢ e ≡ .sort u : A) :
+    ∃ u', Γ ⊢ e ⤳* .sort u' ∧ u' ≈ u := by
+  have ⟨_, _, e', _, h1, h2, h3⟩ := H.church_rosser hΓ
+  cases (h2.standard hΓ H.hasType.2).sort_l
+  have hu := H.hasType.2.sort_inv henv
+  obtain ⟨v, rfl, a1⟩ : ∃ v, e' = sort v ∧ v ≈ u := by
+    cases h3 with
+    | refl => exact ⟨_, rfl, rfl⟩
+    | sortDF _ _ h => exact ⟨_, rfl, h⟩
+    | etaL h => cases ((HasType.sort hu).uniqU henv hΓ h).sort_forallE_inv henv hΓ
+    | proofIrrel h1 _ h3 =>
+      have := h1.defeqU_l henv hΓ ((HasType.sort hu).uniqU henv hΓ h3).symm
+      have := ((HasType.sort (by exact hu)).uniqU henv hΓ this).sort_inv henv hΓ
+      cases congrFun this []
+  let .sort h1 := h1.standard hΓ H.hasType.1
+  exact ⟨_, h1, a1⟩
+
+variable! (hΓ : OnCtx Γ (IsType env univs)) in
+theorem IsDefEq.reduce_forallE (H : Γ ⊢ e ≡ .forallE A B : V) :
+    ∃ A' B', Γ ⊢ e ⤳* .forallE A' B' := by
+  have ⟨_, _, e', _, h1, h2, h3⟩ := H.church_rosser hΓ
+  obtain ⟨A₁, B₁, rfl, eA, eB⟩ := (h2.standard hΓ H.hasType.2).forallE_l
+  have ⟨⟨_, hA⟩, _, hB⟩ := H.hasType.2.forallE_inv henv
+  have hA₁ := eA.parRedS.defeq hΓ hA
+  have hB₁ := eB.parRedS.hasType (by exact ⟨hΓ, _, hA⟩) hB |>.defeq_l henv hA₁
+  obtain ⟨_, _, rfl⟩ : ∃ A' B', e' = .forallE A' B' := by
+    cases h3 with
+    | refl
+    | forallEDF _ _ h => exact ⟨_, _, rfl⟩
+    | etaL h => cases ((hA₁.hasType.2.forallE hB₁).uniqU henv hΓ h).sort_forallE_inv henv hΓ
+    | proofIrrel h1 _ h3 =>
+      have := h1.defeqU_l henv hΓ ((hA₁.hasType.2.forallE hB₁).uniqU henv hΓ h3).symm
+      have := ((HasType.sort (by exact this.sort_inv henv)).uniqU henv hΓ this).sort_inv henv hΓ
+      cases congrFun this []
+  let .forallE h1 .. := h1.standard hΓ H.hasType.1
+  exact ⟨_, _, h1⟩
